lib/FastMap: refactor convs; renaming; juggle function arguments
Complex conversions have been refactored to the new utility conv_at,
which is easier to use and has better error detection.

Name changes: “*_to_map” naming scheme changed to more descriptive
“*_to_lookup_list”.

Key transformer argument is now the first argument to tree_lookup and
friends, which matches functional programming conventions.

lib/FastMap.thy
@@ -29,9 +29,11 @@ text \<open>
 (*
  * TODO:
  *
- *   • Storing the (large) auxilliary theorems with Local_Theory.notes
- *     seems to take quadratic time. Investigate this, or work around
- *     it by hiding the map data behind additional constants.
+ *   • Storing the auxilliary list theorems with Local_Theory.notes
+ *     takes quadratic time. Unfortunately, this seems to be a problem
+ *     deep inside the Isabelle implementation. One might try to wrap
+ *     the lists in new constants, but Local_Theory.define also takes
+ *     quadratic time.
  *
  *   • Still a bit slower than the StaticFun package. Streamline the
  *     rulesets and proofs.
@@ -47,6 +49,11 @@ text \<open>
  *   • The injectivity prover currently hardcodes inj_def into the
  *     simpset. This should be changed at some point, probably by
  *     asking the user to prove it beforehand.
+ *
+ *   • The key ordering prover is currently hardcoded to simp_tac;
+ *     this should also be generalised. On the other hand, the user
+ *     could work around this by manually supplying a simpset with
+ *     precisely the needed theorems.
  *
  *   • Using the simplifier to evaluate tree lookups is still quite
  *     slow because it looks at the entire tree term (even though
@@ -73,17 +80,19 @@ text \<open>
   Binary lookup tree. This is largely an implementation detail, so we
   choose the structure to make automation easier (e.g. separate fields
   for the key and value).
+
+  We could reuse HOL.Tree instead, but the proofs would need changing.
 \<close>
 datatype ('k, 'v) Tree = Leaf | Node 'k 'v "('k, 'v) Tree" "('k, 'v) Tree"
 
 primrec
-  lookup_tree :: "('k, 'v) Tree \<Rightarrow> ('k \<Rightarrow> 'ok :: linorder) \<Rightarrow> 'k \<Rightarrow> 'v option"
+  lookup_tree :: "('k \<Rightarrow> 'ok :: linorder) \<Rightarrow> ('k, 'v) Tree \<Rightarrow> 'k \<Rightarrow> 'v option"
 where
-  "lookup_tree Leaf fn x = None"
-| "lookup_tree (Node k v l r) fn x =
-     (if fn x = fn k then Some v
-      else if fn x < fn k then lookup_tree l fn x
-      else lookup_tree r fn x)"
+  "lookup_tree key Leaf x = None"
+| "lookup_tree key (Node k v l r) x =
+     (if key x = key k then Some v
+      else if key x < key k then lookup_tree key l x
+      else lookup_tree key r x)"
 
 text \<open>
   Predicate for well-formed lookup trees.
@@ -137,7 +146,7 @@ lemma lookup_tree_valid_range:
 
 lemma lookup_tree_valid_in_range:
   "lookup_tree_valid key tree = (True, Some (low, high)) \<Longrightarrow>
-   lookup_tree tree key k = Some v \<Longrightarrow>
+   lookup_tree key tree k = Some v \<Longrightarrow>
    key k \<in> {key low .. key high}"
   apply (induct tree arbitrary: k v low high)
    apply simp
@@ -148,20 +157,21 @@ lemma lookup_tree_valid_in_range:
 lemma lookup_tree_valid_in_range_None:
   "lookup_tree_valid key tree = (True, Some (low, high)) \<Longrightarrow>
    key k \<notin> {key low .. key high} \<Longrightarrow>
-   lookup_tree tree key k = None"
+   lookup_tree key tree k = None"
   using lookup_tree_valid_in_range by fastforce
 
 text \<open>
   Flatten a lookup tree into an assoc-list.
   As long as the tree is well-formed, both forms are equivalent.
 \<close>
-primrec lookup_tree_to_map where
-  "lookup_tree_to_map Leaf = []"
-| "lookup_tree_to_map (Node k v lt rt) = lookup_tree_to_map lt @ [(k, v)] @ lookup_tree_to_map rt"
+primrec lookup_tree_to_list where
+  "lookup_tree_to_list Leaf = []"
+| "lookup_tree_to_list (Node k v lt rt) =
+      lookup_tree_to_list lt @ [(k, v)] @ lookup_tree_to_list rt"
 
-lemma lookup_tree_to_map_range:
+lemma lookup_tree_to_list_range:
   "lookup_tree_valid key tree = (True, Some (low, high)) \<Longrightarrow>
-   (k, v) \<in> set (lookup_tree_to_map tree) \<Longrightarrow>
+   (k, v) \<in> set (lookup_tree_to_list tree) \<Longrightarrow>
    key k \<in> {key low .. key high}"
   apply (induct tree arbitrary: k v low high)
    apply simp
@@ -171,23 +181,23 @@ lemma lookup_tree_to_map_range:
 
 lemma lookup_tree_dom_distinct_sorted_:
   "fst (lookup_tree_valid key tree) \<Longrightarrow>
-   distinct (lookup_tree_to_map tree) \<and> sorted (map (key o fst) (lookup_tree_to_map tree))"
+   distinct (lookup_tree_to_list tree) \<and> sorted (map (key o fst) (lookup_tree_to_list tree))"
   apply (induct tree)
    apply simp
   apply (fastforce simp: sorted_append
                    split: prod.splits option.splits if_splits
                    dest: lookup_tree_valid_empty lookup_tree_valid_range
-                         lookup_tree_valid_in_range lookup_tree_to_map_range
+                         lookup_tree_valid_in_range lookup_tree_to_list_range
                    elim: lookup_tree_valid_in_range_None)
   done
 
 lemmas lookup_tree_dom_distinct = lookup_tree_dom_distinct_sorted_[THEN conjunct1]
 lemmas lookup_tree_dom_sorted = lookup_tree_dom_distinct_sorted_[THEN conjunct2]
 
-(* The goal is eta-expanded and flipped, which seems to help the proof *)
-lemma lookup_tree_to_map_of_:
+(* This goal is eta-expanded and flipped, which seems to help its proof *)
+lemma lookup_tree_to_list_of_:
   "fst (lookup_tree_valid key tree) \<Longrightarrow>
-   map_of (map (apfst key) (lookup_tree_to_map tree)) (key k) = lookup_tree tree key k"
+   map_of (map (apfst key) (lookup_tree_to_list tree)) (key k) = lookup_tree key tree k"
   apply (induct tree arbitrary: k)
    apply simp
   (* this big blob just does case distinctions of both subtrees and
@@ -200,11 +210,11 @@ lemma lookup_tree_to_map_of_:
   done
 
 (* Standard form of above *)
-lemma lookup_tree_to_map_of:
+lemma lookup_tree_to_list_of:
   "fst (lookup_tree_valid key tree) \<Longrightarrow>
-   lookup_tree tree key = map_of (map (apfst key) (lookup_tree_to_map tree)) o key"
+   lookup_tree key tree = map_of (map (apfst key) (lookup_tree_to_list tree)) o key"
   apply (rule ext)
-  apply (simp add: lookup_tree_to_map_of_)
+  apply (simp add: lookup_tree_to_list_of_)
   done
 
 lemma map_of_key:
@@ -215,20 +225,20 @@ lemma map_of_key:
   apply (clarsimp simp: inj_def dom_def)
   done
 
-lemma lookup_tree_to_map_of_distinct:
+lemma lookup_tree_to_list_of_distinct:
   "\<lbrakk> fst (lookup_tree_valid key tree);
-     lookup_tree_to_map tree = binds;
-     lookup_tree tree key = map_of (map (apfst key) binds) o key
+     lookup_tree_to_list tree = binds;
+     lookup_tree key tree = map_of (map (apfst key) binds) o key
    \<rbrakk> \<Longrightarrow> distinct (map (key o fst) binds)"
   apply (drule sym[where t = binds])
   apply clarsimp
   apply (thin_tac "binds = _")
   apply (induct tree)
    apply simp
-  apply (fastforce simp: map_add_def lookup_tree_to_map_of
+  apply (fastforce simp: map_add_def lookup_tree_to_list_of
                    split: prod.splits option.splits if_splits
                    dest: lookup_tree_valid_empty lookup_tree_valid_range
-                         lookup_tree_valid_in_range lookup_tree_to_map_range
+                         lookup_tree_valid_in_range lookup_tree_to_list_range
                    elim: lookup_tree_valid_in_range_None)
   done
 
@@ -241,13 +251,13 @@ lemma distinct_inj:
 
 (* Top-level rule for converting to lookup list.
    We add a distinctness assertion for inferring the range of values. *)
-lemma lookup_tree_to_map_of_gen:
+lemma lookup_tree_to_list_of_gen:
   "\<lbrakk> inj key;
      fst (lookup_tree_valid key tree);
-     lookup_tree_to_map tree = binds
-   \<rbrakk> \<Longrightarrow> lookup_tree tree key = map_of binds \<and> distinct (map fst binds)"
-  using lookup_tree_to_map_of
-  apply (fastforce intro: lookup_tree_to_map_of_distinct
+     lookup_tree_to_list tree = binds
+   \<rbrakk> \<Longrightarrow> lookup_tree key tree = map_of binds \<and> distinct (map fst binds)"
+  using lookup_tree_to_list_of
+  apply (fastforce intro: lookup_tree_to_list_of_distinct
                    simp: map_of_key distinct_inj)
   done
 
@@ -295,15 +305,15 @@ lemma list_all_dest:
 
 (* Install lookup rules that don't depend on if_cong/if_weak_cong setup *)
 lemma lookup_tree_simps':
-  "lookup_tree Leaf fn x = None"
-  "fn x = fn y \<Longrightarrow> lookup_tree (Node y v l r) fn x = Some v"
-  "fn x < fn y \<Longrightarrow> lookup_tree (Node y v l r) fn x = lookup_tree l fn x"
-  "fn x > fn y \<Longrightarrow> lookup_tree (Node y v l r) fn x = lookup_tree r fn x"
+  "lookup_tree key Leaf x = None"
+  "key x = key k \<Longrightarrow> lookup_tree key (Node k v l r) x = Some v"
+  "key x < key k \<Longrightarrow> lookup_tree key (Node k v l r) x = lookup_tree key l x"
+  "key x > key k \<Longrightarrow> lookup_tree key (Node k v l r) x = lookup_tree key r x"
   by auto
 end
 
-declare FastMap.lookup_tree_simps'[simp]
 declare FastMap.lookup_tree.simps[simp del]
+declare FastMap.lookup_tree_simps'[simp]
 
 ML \<open>
 structure FastMap = struct
@@ -313,6 +323,13 @@ fun mk_optionT typ = Type ("Option.option", [typ])
 fun dest_optionT (Type ("Option.option", [typ])) = typ
   | dest_optionT t = raise TYPE ("dest_optionT", [t], [])
 
+(* O(1) version of thm RS @{thm eq_reflection} *)
+fun then_eq_reflection thm = let
+  val (x, y) = Thm.dest_binop (Thm.dest_arg (Thm.cprop_of thm));
+  val cT = Thm.ctyp_of_cterm x;
+  val rule = @{thm eq_reflection} |> Thm.instantiate' [SOME cT] [SOME x, SOME y];
+  in Thm.implies_elim rule thm end;
+
 val lhs_conv = Conv.fun_conv o Conv.arg_conv
 val rhs_conv = Conv.arg_conv
 (* first order rewr_conv *)
@@ -320,10 +337,57 @@ fun fo_rewr_conv rule ct = let
   val (pure_eq, eqn) =
         ((true, Thm.instantiate (Thm.first_order_match (Thm.lhs_of rule, ct)) rule)
          handle TERM _ =>
-           (false, Thm.instantiate (Thm.first_order_match (fst (Thm.dest_binop (Thm.dest_arg (Thm.cprop_of rule))), ct)) rule))
+           (false, Thm.instantiate (Thm.first_order_match
+                      (fst (Thm.dest_binop (Thm.dest_arg (Thm.cprop_of rule))), ct)) rule))
         handle Pattern.MATCH => raise CTERM ("fo_rewr_conv", [Thm.cprop_of rule, ct]);
-  in if pure_eq then eqn else eqn RS @{thm eq_reflection} end;
+  in if pure_eq then eqn else then_eq_reflection eqn end;
 fun fo_rewrs_conv rules = Conv.first_conv (map fo_rewr_conv rules);
+
+(* Evaluate a term with rewrite rules. Unlike the simplifier, this
+ * does only one top-down pass, but that's enough for tasks like
+ * pushing List.map through a list. Also runs much faster. *)
+fun fo_topdown_rewr_conv rules ctxt =
+      Conv.top_conv (K (Conv.try_conv (fo_rewrs_conv rules))) ctxt
+
+(* Allow recursive conv in cv2, deferred by function application *)
+infix 1 then_conv'
+fun (cv1 then_conv' cv2) ct =
+  let
+    val eq1 = cv1 ct;
+    val eq2 = cv2 () (Thm.rhs_of eq1);
+  in
+    if Thm.is_reflexive eq1 then eq2
+    else if Thm.is_reflexive eq2 then eq1
+    else Thm.transitive eq1 eq2
+  end;
+
+(* Helper that makes it easier to describe where to apply a conv.
+ * This takes a skeleton term and applies the conversion wherever "HERE"
+ * appears in the skeleton *)
+fun conv_at skel conv ctxt ct = let
+  fun mismatch current_skel current_ct =
+    raise TERM ("conv_at mismatch", [current_skel, Thm.term_of current_ct, skel, Thm.term_of ct])
+
+  fun walk (Free ("HERE", _)) ctxt ct = conv ct
+    | walk (skel as skel_f $ skel_x) ctxt ct =
+        (case Thm.term_of ct of
+            f $ x => Conv.combination_conv (walk skel_f ctxt) (walk skel_x ctxt) ct
+          | _ => mismatch skel ct)
+    | walk (skel as Abs (_, _, skel_body)) ctxt ct =
+        (case Thm.term_of ct of
+            Abs _ => Conv.abs_conv (fn (v, ctxt') => walk skel_body ctxt') ctxt ct
+          | _ => mismatch skel ct)
+    (* Also check that Consts match the skeleton pattern *)
+    | walk (skel as Const (skel_name, _)) ctxt ct =
+        if (case Thm.term_of ct of Const (name, _) => name = skel_name | _ => false)
+        then Thm.reflexive ct
+        else mismatch skel ct
+    (* Default case *)
+    | walk _ ctxt ct = Thm.reflexive ct
+  in walk skel ctxt ct end
+
+fun gconv_at_tac pat conv ctxt = Conv.gconv_rule (conv_at pat conv ctxt) 1 #> Seq.succeed
+
 
 (* Tree builder code, copied from StaticFun *)
 
@@ -337,7 +401,7 @@ fun build_tree' _ mk_leaf [] = mk_leaf
         (build_tree' mk_node mk_leaf zs)
   end
 
-fun build_tree ord xs = case xs of [] => error "build_tree : empty"
+fun build_tree xs = case xs of [] => error "build_tree : empty"
   | (idx, v) :: _ => let
     val idxT = fastype_of idx
     val vT = fastype_of v
@@ -346,18 +410,21 @@ fun build_tree ord xs = case xs of [] => error "build_tree : empty"
     val node = Const (@{const_name FastMap.Node},
         idxT --> vT --> treeT --> treeT --> treeT)
     fun mk_node a b l r = node $ a $ b $ l $ r
-    val lookup = Const (@{const_name FastMap.lookup_tree},
-        treeT --> fastype_of ord --> idxT
-            --> Type (@{type_name option}, [vT]))
   in
-    lookup $ (build_tree' mk_node mk_leaf xs) $ ord
+    build_tree' mk_node mk_leaf xs
   end
 
-fun define_partial_map_tree name mappings ord ctxt = let
-    val tree = build_tree ord mappings
-  in Local_Theory.define
-    ((name, NoSyn), ((Thm.def_binding name, []), tree)) ctxt
-    |> apfst (apsnd snd)
+fun define_partial_map_tree map_name mappings ord_term ctxt = let
+    val (idxT, vT) = apply2 fastype_of (hd mappings)
+    val treeT = Type (@{type_name FastMap.Tree}, [idxT, vT])
+    val lookup = Const (@{const_name FastMap.lookup_tree},
+                        fastype_of ord_term --> treeT --> idxT
+                            --> Type (@{type_name option}, [vT]))
+    val map_term = lookup $ ord_term $ build_tree mappings
+    val ((map_const, (_, map_def)), ctxt) =
+          Local_Theory.define ((map_name, NoSyn), ((Thm.def_binding map_name, []), map_term)) ctxt
+  in
+    ((map_const, map_def), ctxt)
   end
 
 (* Prove key ordering theorems. This lets us issue precise error messages
@@ -372,12 +439,12 @@ fun prove_key_ord_thms tree_name keyT mappings get_key simp_ctxt ctxt =
            val prop = Const (@{const_name less}, keyT --> keyT --> HOLogic.boolT) $
                             (get_key $ k1) $ (get_key $ k2)
                       |> HOLogic.mk_Trueprop;
-           val thm = case try (Goal.prove ctxt [] [] prop) (K solver) of
-                        SOME x => x
-                      | _ => raise TERM (tree_name ^ ": failed to prove less-than ordering for keys #" ^
-                                         string_of_int i ^ ", #" ^ string_of_int (i + 1),
-                                         [prop]);
-         in thm end)
+           in case try (Goal.prove ctxt [] [] prop) (K solver) of
+                  SOME x => x
+                | _ => raise TERM (tree_name ^ ": failed to prove less-than ordering for keys #" ^
+                                   string_of_int i ^ ", #" ^ string_of_int (i + 1),
+                                   [prop])
+           end)
   end;
 
 (* Prove lookup_tree_valid *)
@@ -388,109 +455,118 @@ fun prove_tree_valid tree_name mappings kT keyT tree_term get_key simp_ctxt ctxt
     val tree_valid_prop =
           HOLogic.mk_Trueprop (
             Const (@{const_name fst}, valid_resultT --> HOLogic.boolT) $
-            (Const (@{const_name FastMap.lookup_tree_valid}, (kT --> keyT) --> treeT --> valid_resultT) $
+            (Const (@{const_name FastMap.lookup_tree_valid},
+                    (kT --> keyT) --> treeT --> valid_resultT) $
                get_key $ tree_term))
     val solver = simp_tac (put_simpset HOL_basic_ss ctxt
-                           addsimps (@{thms prod.sel FastMap.lookup_tree_valid_simps'} @ key_ord_thms)) 1
+                           addsimps (@{thms prod.sel FastMap.lookup_tree_valid_simps'} @
+                                     key_ord_thms)) 1
   in Goal.prove ctxt [] [] tree_valid_prop (K solver) end
 
 fun solve_simp_tac name ctxt = SUBGOAL (fn (t, i) =>
       (simp_tac ctxt THEN_ALL_NEW SUBGOAL (fn (t', _) =>
           raise TERM (name ^ ": unsolved", [t, t']))) i)
 
-fun convert_tree_to_map kT valT mappings lookup_const tree_def tree_valid_thm simp_ctxt ctxt = let
-  val lookupT = fastype_of lookup_const
+fun convert_to_lookup_list kT valT mappings map_const map_def tree_valid_thm simp_ctxt ctxt = let
+  val lookupT = fastype_of map_const
   (* map_eq = "<tree_const> = map_of <mappings>" *)
   val bindT = HOLogic.mk_prodT (kT, valT)
-  val mapping_list = HOLogic.mk_list bindT (map HOLogic.mk_prod mappings)
-  val map_eq = HOLogic.mk_eq (lookup_const, Const (@{const_name map_of}, HOLogic.listT bindT --> lookupT) $ mapping_list)
+  val lookup_list = HOLogic.mk_list bindT (map HOLogic.mk_prod mappings)
+  val map_of_Const = Const (@{const_name map_of}, HOLogic.listT bindT --> lookupT)
+  val map_eq = HOLogic.mk_eq (map_const, map_of_Const $ lookup_list)
   (* distinct_pred = "distinct (map fst <mappings>)" *)
   val distinct_pred =
         Const (@{const_name distinct}, HOLogic.listT kT --> HOLogic.boolT) $
           (Const (@{const_name map}, (bindT --> kT) --> HOLogic.listT bindT --> HOLogic.listT kT) $
              Const (@{const_name fst}, bindT --> kT) $
-             mapping_list)
+             lookup_list)
   val convert_prop = HOLogic.mk_Trueprop (
         HOLogic.mk_conj (map_eq, distinct_pred)
         )
-  fun TIMED desc tac = fn st => Seq.make (K (Timing.timeap_msg ("tactic timing for " ^ desc) (fn () => Seq.pull (tac st)) ()))
+  fun TIMED desc tac = fn st =>
+        Seq.make (K (Timing.timeap_msg ("tactic timing for " ^ desc)
+                          (fn () => Seq.pull (tac st)) ()))
 
-  val lookup_tree_to_map_eval = let
-    (* allow recursive conv in cv2, deferred by function application *)
-    infix 1 then_conv'
-    fun (cv1 then_conv' cv2) ct =
-      let
-        val eq1 = cv1 ct;
-        val eq2 = cv2 () (Thm.rhs_of eq1);
-      in
-        if Thm.is_reflexive eq1 then eq2
-        else if Thm.is_reflexive eq2 then eq1
-        else Thm.transitive eq1 eq2
-      end;
+  val append_basecase = @{thm append.simps(1)}
+  val append_rec = @{thm append.simps(2)}
+  val lookup_tree_to_list_basecase = @{thm FastMap.lookup_tree_to_list.simps(1)}
+  val lookup_tree_to_list_rec = @{thm FastMap.lookup_tree_to_list.simps(2)[simplified append.simps]}
 
+  val lookup_tree_to_list_eval = let
     fun append_conv () =
-            fo_rewr_conv @{thm append.simps(1)} else_conv
-            (fo_rewr_conv @{thm append.simps(2)} then_conv'
+            fo_rewr_conv append_basecase else_conv
+            (fo_rewr_conv append_rec then_conv'
              (fn () => rhs_conv (append_conv ())))
     fun to_map_conv () =
-            fo_rewr_conv @{thm FastMap.lookup_tree_to_map.simps(1)} else_conv
-            (fo_rewr_conv @{thm FastMap.lookup_tree_to_map.simps(2)[simplified append.simps]} then_conv'
+            fo_rewr_conv lookup_tree_to_list_basecase else_conv
+            (fo_rewr_conv lookup_tree_to_list_rec then_conv'
              (fn () => lhs_conv (to_map_conv ())) then_conv'
              (fn () => rhs_conv (rhs_conv (to_map_conv ()))) then_conv
              append_conv ())
   in to_map_conv () end
 
   val solver =
-        TIMED "unfold" (Conv.gconv_rule (Conv.arg_conv (lhs_conv (lhs_conv (K tree_def)))) 1 #> Seq.succeed) THEN
-        TIMED "main rule" (resolve_tac ctxt @{thms FastMap.lookup_tree_to_map_of_gen} 1) THEN
-          TIMED "solve inj" (solve_simp_tac "convert_tree_to_map" (simp_ctxt ctxt @{thms simp_thms} @{thms inj_def}) 1) THEN
-         TIMED "resolve valid" (resolve_tac ctxt [tree_valid_thm] 1) THEN
-        TIMED "convert tree" (Conv.gconv_rule (Conv.arg_conv (lhs_conv lookup_tree_to_map_eval)) 1 #> Seq.succeed) THEN
+        TIMED "unfold" (gconv_at_tac @{term "Trueprop (HERE = map_of dummy1 \<and> dummy2)"}
+                                     (K map_def) ctxt)
+        THEN
+        TIMED "main rule" (resolve_tac ctxt @{thms FastMap.lookup_tree_to_list_of_gen} 1)
+        THEN
+          TIMED "solve inj" (solve_simp_tac "solve inj"
+                              (simp_ctxt ctxt @{thms simp_thms} @{thms inj_def}) 1)
+          THEN
+         TIMED "resolve valid" (resolve_tac ctxt [tree_valid_thm] 1)
+         THEN
+        TIMED "convert tree" (gconv_at_tac @{term "Trueprop (HERE = dummy1)"}
+                                           lookup_tree_to_list_eval ctxt)
+        THEN
         resolve_tac ctxt @{thms refl} 1
   val convert_thm = Goal.prove ctxt [] [] convert_prop (K solver)
   in convert_thm end
 
 (* Obtain domain and range from lookup list *)
-fun domain_range_common dom_ran_const xT xs lookup_const tree_map_eqn intro_conv_tac ctxt = let
-  val lookupT = fastype_of lookup_const
+fun domain_range_common dom_ran_const xT xs map_const lookup_list_eqn intro_conv_tac ctxt = let
+  val mapT = fastype_of map_const
   val prop = HOLogic.mk_Trueprop (
         HOLogic.mk_eq (
-          Const (dom_ran_const, lookupT --> HOLogic.mk_setT xT) $ lookup_const,
+          Const (dom_ran_const, mapT --> HOLogic.mk_setT xT) $ map_const,
           Const (@{const_name set}, HOLogic.listT xT --> HOLogic.mk_setT xT) $
             (HOLogic.mk_list xT xs)
         ))
-  val tree_map_eqn' = tree_map_eqn RS @{thm eq_reflection}
-  val map_eqns = @{thms list.map prod.sel}
+  val lookup_list_eqn' = then_eq_reflection lookup_list_eqn
+  val map_fst_snd_conv = fo_topdown_rewr_conv @{thms list.map prod.sel} ctxt
   val solver =
-        (Conv.gconv_rule (Conv.arg_conv (lhs_conv (Conv.arg_conv (K tree_map_eqn')))) 1 #> Seq.succeed) THEN
-        intro_conv_tac THEN
-        (Conv.gconv_rule (Conv.arg_conv (lhs_conv (
-             Conv.top_conv (K (Conv.try_conv (fo_rewrs_conv map_eqns))) ctxt
-           ))) 1 #> Seq.succeed) THEN
+        (gconv_at_tac @{term "Trueprop (dom_ran_dummy1 HERE = dummy2)"}
+                      (K lookup_list_eqn') ctxt)
+        THEN
+        intro_conv_tac
+        THEN
+        gconv_at_tac @{term "Trueprop (HERE = dummy1)"} map_fst_snd_conv ctxt
+        THEN
         resolve_tac ctxt @{thms refl} 1
   in Goal.prove ctxt [] [] prop (K solver) end;
 
-fun tree_domain kT mappings lookup_const tree_map_eqn ctxt =
+fun tree_domain kT mappings map_const lookup_list_eqn ctxt =
   domain_range_common
-    @{const_name dom} kT (map fst mappings) lookup_const tree_map_eqn
+    @{const_name dom} kT (map fst mappings) map_const lookup_list_eqn
     (* like (subst dom_map_of_conv_list) but faster *)
     (resolve_tac ctxt @{thms FastMap.dom_map_of_conv_list[THEN trans]} 1)
     ctxt;
 
-fun tree_range valT mappings lookup_const tree_map_eqn map_distinct_thm ctxt =
+fun tree_range valT mappings map_const lookup_list_eqn map_distinct_thm ctxt =
   domain_range_common
-    @{const_name ran} valT (map snd mappings) lookup_const tree_map_eqn
+    @{const_name ran} valT (map snd mappings) map_const lookup_list_eqn
     (* like (subst ran_map_of_conv_list) but faster *)
     (resolve_tac ctxt @{thms FastMap.ran_map_of_conv_list[THEN trans]} 1 THEN
      resolve_tac ctxt [map_distinct_thm] 1)
     ctxt;
+
 
 (* Choosing names for the const and its theorems. The constant will be named with
    map_name; Local_Theory.define may also add extra names (e.g. <map_name>_def) *)
 type name_opts = {
     map_name: string,
     tree_valid_thm: string,
-    tree_map_eqn: string,
+    to_lookup_list: string,
     keys_distinct_thm: string,
     lookup_thms: string,
     domain_thm: string,
@@ -500,7 +576,7 @@ type name_opts = {
 fun name_opts_default (map_name: string): name_opts = {
     map_name = map_name,
     tree_valid_thm = map_name ^ "_tree_valid",
-    tree_map_eqn = map_name ^ "_tree_to_map",
+    to_lookup_list = map_name ^ "_to_lookup_list",
     keys_distinct_thm = map_name ^ "_keys_distinct",
     lookup_thms = map_name ^ "_lookups",
     domain_thm = map_name ^ "_domain",
@@ -519,18 +595,22 @@ fun define_map
       then put_simpset HOL_basic_ss ctxt addsimps (basic_simps @ extra_simps @ more_simps)
       else ctxt addsimps (extra_simps @ more_simps)
 
+    val (kT, keyT) = dest_funT (fastype_of get_key)
+    val valT = fastype_of (snd (hd mappings))
+
     val _ = tracing (#map_name name_opts ^ ": defining tree")
     val start = Timing.start ()
-    val ((lookup_const, tree_def), ctxt) =
-            define_partial_map_tree (Binding.name (#map_name name_opts)) mappings get_key ctxt
-    val (tree_const, _ $ tree_term $ _) = Logic.dest_equals (Thm.prop_of tree_def)
-    val (kT, keyT) = dest_funT (fastype_of get_key)
-    val valT = dest_optionT (snd (dest_funT (fastype_of tree_const)))
+    val ((map_const, map_def), ctxt) =
+            define_partial_map_tree
+                (Binding.name (#map_name name_opts))
+                mappings get_key ctxt
     val _ = tracing ("  done: " ^ Timing.message (Timing.result start))
 
     val _ = tracing (#map_name name_opts ^ ": proving tree is well-formed")
     val start = Timing.start ()
-    val tree_valid_thm = prove_tree_valid (#map_name name_opts) mappings kT keyT tree_term get_key simp_ctxt ctxt
+    val _ $ _ $ tree_term = Thm.term_of (Thm.rhs_of map_def)
+    val tree_valid_thm =
+          prove_tree_valid (#map_name name_opts) mappings kT keyT tree_term get_key simp_ctxt ctxt
     val (_, ctxt) = ctxt |> Local_Theory.notes
         [((Binding.name (#tree_valid_thm name_opts), []), [([tree_valid_thm], [])])]
     val _ = tracing ("  done: " ^ Timing.message (Timing.result start))
@@ -538,24 +618,30 @@ fun define_map
     val _ = tracing (#map_name name_opts ^ ": converting tree to map")
     val start = Timing.start ()
     val convert_thm =
-          convert_tree_to_map kT valT mappings lookup_const tree_def tree_valid_thm simp_ctxt ctxt
-    val [tree_map_eqn, map_distinct_thm] = HOLogic.conj_elims ctxt convert_thm
+          convert_to_lookup_list kT valT mappings map_const map_def tree_valid_thm simp_ctxt ctxt
+    val [lookup_list_eqn, map_distinct_thm] = HOLogic.conj_elims ctxt convert_thm
     val _ = tracing ("  done: " ^ Timing.message (Timing.result start))
     val _ = tracing (#map_name name_opts ^ ": storing map and distinctness theorems")
     val start = Timing.start ()
     val (_, ctxt) = ctxt |> Local_Theory.notes
-        [((Binding.name (#tree_map_eqn name_opts), []), [([tree_map_eqn], [])]),
+        [((Binding.name (#to_lookup_list name_opts), []), [([lookup_list_eqn], [])]),
          ((Binding.name (#keys_distinct_thm name_opts), []), [([map_distinct_thm], [])])]
     val _ = tracing ("  done: " ^ Timing.message (Timing.result start))
 
     val _ = tracing (#map_name name_opts ^ ": obtaining lookup rules")
     val start = Timing.start ()
+    fun dest_list_all_conv () =
+          fo_rewr_conv @{thm FastMap.list_all_dest(1)} else_conv
+          (fo_rewr_conv @{thm FastMap.list_all_dest(2)} then_conv'
+           (fn () => rhs_conv (dest_list_all_conv())))
     val combined_lookup_thm =
           (convert_thm RS @{thm FastMap.map_of_lookups})
-          |> Conv.fconv_rule (Conv.top_conv (K (Conv.try_conv (fo_rewrs_conv @{thms FastMap.list_all_dest}))) ctxt)
+          |> Conv.fconv_rule (conv_at @{term "Trueprop HERE"} (dest_list_all_conv ()) ctxt)
     val _ = tracing ("  splitting... " ^ Timing.message (Timing.result start))
-    val lookup_thms = HOLogic.conj_elims ctxt combined_lookup_thm
-                      |> map (Conv.fconv_rule (Conv.arg_conv (Conv.rewr_conv @{thm prod.case[THEN eq_reflection]})))
+    val lookup_thms =
+          HOLogic.conj_elims ctxt combined_lookup_thm
+          |> map (Conv.fconv_rule (conv_at @{term "Trueprop HERE"}
+                                     (fo_rewr_conv @{thm prod.case[THEN eq_reflection]}) ctxt))
 
     val _ = if length lookup_thms = length mappings then () else
               raise THM ("wrong number of lookup thms: " ^ string_of_int (length lookup_thms) ^
@@ -569,9 +655,9 @@ fun define_map
     val _ = tracing (#map_name name_opts ^ ": getting domain and range")
     val start = Timing.start ()
     val domain_thm = timeap_msg "  calculate domain"
-            (tree_domain kT mappings lookup_const tree_map_eqn) ctxt
+            (tree_domain kT mappings map_const lookup_list_eqn) ctxt
     val range_thm = timeap_msg "  calculate range"
-            (tree_range valT mappings lookup_const tree_map_eqn map_distinct_thm) ctxt
+            (tree_range valT mappings map_const lookup_list_eqn map_distinct_thm) ctxt
     val (_, ctxt) = ctxt |> Local_Theory.notes
         [((Binding.name (#domain_thm name_opts), []), [([domain_thm], [])]),
          ((Binding.name (#range_thm name_opts), []), [([range_thm], [])])]
